updated the inlined documentation for AFP submission. Main additions in Airplane.thy by pasting in main explanation from the journal/arxive version.

AirInsider.thy
@@ -1,45 +1,106 @@
 section "Insider Framework"
+text \<open>In the Isabelle/HOL theory for Insiders, one expresses policies over
+actions @{text \<open>get, move, eval\<close>}, and @{text \<open>put\<close>}.\<close>
+subsection \<open>Actors and actions\<close>
+text \<open>The theory Airinsider is an instance of the Insider framework for the case study
+     of airplane insiders. Although the Isabelle Insider framework is a generic framework
+     the actual semantics of the actions is specific to applications. Therefore we use here
+     an "instance" of the framework in the form of a theory "Airinsider" but the main part of 
+     definitions and declarations is the same.\<close>
 theory AirInsider
-imports MC
+  imports MC
 begin
-datatype action = get | move | eval |put
+text \<open>An actor may be enabled to 
+\begin{itemize}
+\item @{text \<open>get\<close>} data or physical items, like keys,
+\item @{text \<open>move\<close>} to a location,
+\item @{text \<open>eval\<close>} a program,
+\item @{text \<open>put\<close>} data at locations or physical items -- like airplanes --
+``to the ground''.
+\end{itemize}
+The precise semantics of these actions is refined in the state transition 
+rules for the concrete infrastructure.
+The framework abstracts from concrete data -- actions have no parameters:\<close>
+datatype action = get | move | eval | put
 
-text \<open>We use an abstract type declaration actor that can later be instantiated by a more 
+text \<open>The human component is the {\it Actor} which is represented by an abstract
+type @{text \<open>actor\<close>} and a function @{text \<open>Actor\<close>}
+that creates elements of that type from identities (of type @{text \<open>string\<close>}):
+
+We use an abstract type declaration actor that can later be instantiated by a more
       concrete type.\<close>
 typedecl actor 
-consts Actor :: "string \<Rightarrow> actor" 
-text \<open>Alternatives to the type declaration do not work.
-
-context
-  fixes Abs Rep actor
-  assumes td: "type\_definition Abs Rep actor"
-begin
-definition Actor where "Actor = Abs"
-...doesn't work for replacing the actor typedecl because 
-in "type\_definition" above the "actor" is a set not a type!
-So can't be used for our purposes. 
-Trying a locale instead for polymorphic type Actor 
-locale ACT =
-  fixes Actor :: "string => 'actor"
-begin ...
-That is a nice idea and works quite far but clashes with the generic
-state\_transition later (it's not possible to instantiate within a locale
-and outside it we cannot instantiate "'a infrastructure" to state (clearly 
-an abstract thing as an instance is strange)\<close>
-
 type_synonym identity = string
-type_synonym  policy = "((actor \<Rightarrow> bool) * action set)"
+consts Actor :: "identity \<Rightarrow> actor" 
+text \<open>Note that it would seem more natural and simpler to just 
+define @{text \<open>actor\<close>} as a datatype over identities with a constructor @{text \<open>Actor\<close>}
+instead of a simple constant together with a type declaration like, for example,
+in the Isabelle inductive approach to security protocol verification \cite{pau:97, pau:98}. 
+This would, however, make the constructor @{text \<open>Actor\<close>} an injective function
+by the underlying foundation of datatypes therefore excluding the fine
+grained modelling that is at the core of the insider definition:
+In fact, it defines the function @{text \<open>Actor\<close>} to be injective
+for all except insiders and explicitly enables insiders to have
+different roles by identifying @{text \<open>Actor\<close>} images.
+
+Alternatives to the type declaration do not work.
+
+@{text \<open>context
+
+  fixes Abs Rep actor
+
+  assumes td: "type_definition Abs Rep actor"
+
+begin
+
+definition Actor where "Actor = Abs"
+\<close>}
+...doesn't work as an alternative to the actor @{term \<open>typedecl\<close>} because 
+in @{text \<open>type_definition\<close>} above the @{text \<open>actor\<close>} is a set not a type!
+So can't be used for our purposes. 
+
+Trying a locale instead for polymorphic type Actor is a suggested alternative 
+\cite{mw:09}.
+
+@{text 
+\<open>locale ACT =
+  fixes Actor :: "string \<Rightarrow> 'actor"
+begin ...\<close>
+}
+That is a nice idea and works quite far but clashes with the generic
+@{text \<open>state_transition\<close>} later (it's not possible to instantiate within a locale
+and outside of it we cannot instantiate @{text \<open>'a infrastructure\<close>} to state (clearly 
+an abstract thing as an instance is strange).\<close>
 
 definition ID :: "[actor, string] \<Rightarrow> bool"
 where "ID a s \<equiv> (a = Actor s)"
 
+subsection \<open>Infrastructure graphs and policies\<close>
+text\<open>Actors are contained in an infrastructure graph. An @{text \<open>igraph\<close>} contains
+a set of location pairs representing the topology of the infrastructure
+as a graph of nodes and a list of actor identities associated to each node 
+(location) in the graph.
+Also an @{text \<open>igraph\<close>} associates actors to a pair of string sets by
+a pair-valued function whose first range component is a set describing
+the credentials in the possession of an actor and the second component
+is a set defining the roles the actor can take on. Finally, an  @{text \<open>igraph\<close>} 
+assigns locations to a pair of a string that defines
+the state of the component. 
+Corresponding projection functions for each of these components of an 
+@{text \<open>igraph\<close>} are provided; they are named @{text \<open>gra\<close>} for the actual set of pairs of
+locations, @{text \<open>agra\<close>} for the actor map, @{text \<open>cgra\<close>} for the credentials,
+and @{text \<open>lgra\<close>} for the state of a location and the data at that location.\<close>
 datatype location = Location nat
-
 datatype igraph = Lgraph "(location * location)set" "location \<Rightarrow> identity list"
                          "actor \<Rightarrow> (string list * string list)"  "location \<Rightarrow> string list"
+text \<open>Atomic policies of type @{text \<open>apolicy\<close>}
+describe prerequisites for actions to be granted to actors given by
+pairs of predicates (conditions) and sets of (enabled) actions:\<close>
+type_synonym  apolicy = "((actor \<Rightarrow> bool) * action set)"
+
 datatype infrastructure = 
          Infrastructure "igraph" 
-                        "[igraph, location] \<Rightarrow> policy set" 
+                        "[igraph, location] \<Rightarrow> apolicy set" 
                        
 primrec loc :: "location \<Rightarrow> nat"
 where  "loc(Location n) = n"
@@ -54,19 +115,16 @@ where  "lgra(Lgraph g a c l) = l"
 
 definition nodes :: "igraph \<Rightarrow> location set" 
 where "nodes g == { x. (? y. ((x,y): gra g) | ((y,x): gra g))}"
-
 definition actors_graph :: "igraph \<Rightarrow> identity set"  
 where  "actors_graph g == {x. ? y. y : nodes g \<and> x \<in> set(agra g y)}"
-
 primrec graphI :: "infrastructure \<Rightarrow> igraph"
 where "graphI (Infrastructure g d) = g"
-primrec delta :: "[infrastructure, igraph, location] \<Rightarrow> policy set"
+primrec delta :: "[infrastructure, igraph, location] \<Rightarrow> apolicy set"
 where "delta (Infrastructure g d) = d"
 primrec tspace :: "[infrastructure, actor ] \<Rightarrow> string list * string list"
   where "tspace (Infrastructure g d) = cgra g"
 primrec lspace :: "[infrastructure, location ] \<Rightarrow> string list"
 where "lspace (Infrastructure g d) = lgra g"
-
 definition credentials :: "string list * string list \<Rightarrow> string set"
   where  "credentials lxl \<equiv> set (fst lxl)"
 definition has :: "[igraph, actor * string] \<Rightarrow> bool"
@@ -75,13 +133,26 @@ definition roles :: "string list * string list \<Rightarrow> string set"
   where  "roles lxl \<equiv> set (snd lxl)"
 definition role :: "[igraph, actor * string] \<Rightarrow> bool"
   where "role G ac \<equiv> snd ac \<in> roles(cgra G (fst ac))"
-
 definition isin :: "[igraph,location, string] \<Rightarrow> bool" 
   where "isin G l s \<equiv> s \<in> set(lgra G l)"
-  
+
+subsection \<open>Insider predicate\<close>
+text \<open>The human actor's level is modelled in the Isabelle Insider framework by assigning
+the individual actor's psychological disposition\footnote{Note that the determination of 
+the psychological state of an actor is not done using the formal system. It is up to a 
+psychologist to determine this. However, if for instance, an actor is classified as 
+@{text \<open>disgruntled\<close>} then this may have an influence on what they are allowed to do according 
+to a company policy and this can be formally described and reasoned about in Isabelle.} 
+@{text \<open>actor_state\<close>} to each actor's identity.\<close>
 datatype psy_states = happy | depressed | disgruntled | angry | stressed
 datatype motivations = financial | political | revenge | curious | competitive_advantage | power | peer_recognition
 
+text \<open>The values used for the definition of the types
+@{text \<open>motivations\<close>} and @{text \<open>psy_state\<close>}
+are based on a taxonomy from psychological insider research \cite{nblgcww:14}.
+The transition to become an insider is represented by a {\it Catalyst} that tips the insider 
+over the edge so he acts as an insider formalized as a ``tipping point'' 
+predicate.\<close>
 datatype actor_state = Actor_state "psy_states" "motivations set"
 primrec motivation :: "actor_state \<Rightarrow> motivations set" 
 where "motivation  (Actor_state p m) =  m"
@@ -91,61 +162,88 @@ where "psy_state  (Actor_state p m) = p"
 definition tipping_point :: "actor_state \<Rightarrow> bool" where
   "tipping_point a \<equiv> ((motivation a \<noteq> {}) \<and> (happy \<noteq> psy_state a))"
 
-text \<open>UasI and UasI' are the central predicates allowing to specify Insiders.
-They define which identities can be mapped to the same role by the Actor function.
-For all other identities, Actor is defined as injective on those identities.\<close>
+text \<open>To embed the fact that the attacker is an insider, the actor can then
+impersonate other actors. In the Isabelle Insider framework, the 
+predicate @{text \<open>Insider\<close>} must be used as a {\it locale} assumption
+to enable impersonation for the insider:
+this assumption entails that an insider @{text \<open>Actor ''Eve''\<close>} can act like 
+their alter ego, say @{text \<open>Actor ''Charly''\<close>} within the context of the locale.
+This is realized by the predicate  @{text \<open>UasI\<close>}:
+@{text \<open>UasI\<close>} and @{text \<open>UasI'\<close>} are the central predicates allowing to specify Insiders.
+They define which identities can be mapped to the same role by the @{text \<open>Actor\<close>} function
+(an impersonation predicate "@{text \<open>a\<close>} can act as @{text \<open>b\<close>}").
+For all other identities, @{text \<open>Actor\<close>} is defined as injective on those identities.
+The first one is stronger and allows substitution of the insider in any context; the second 
+one is parameterized over a context predicate to describe this.\<close>
 definition UasI ::  "[identity, identity] \<Rightarrow> bool " 
 where "UasI a b \<equiv> (Actor a = Actor b) \<and> (\<forall> x y. x \<noteq> a \<and> y \<noteq> a \<and> Actor x = Actor y \<longrightarrow> x = y)"
-
-definition UasI' ::  "[actor => bool, identity, identity] \<Rightarrow> bool " 
+definition UasI' ::  "[actor \<Rightarrow> bool, identity, identity] \<Rightarrow> bool " 
 where "UasI' P a b \<equiv> P (Actor b) \<longrightarrow> P (Actor a)"
 
-text \<open>Two versions of Insider predicate corresponding to UasI and UasI'.
-Under the assumption that the tipping point has been reached for a person a
-then a can impersonate all b (take all of b's "roles") where
-the b's are specified by a given set of identities \<close>
+text \<open>Two versions of Insider predicate corresponding to @{text \<open>UasI\<close>} and @{text \<open>UasI'\<close>}
+exist. Under the assumption that the tipping point has been reached for a person @{text \<open>a\<close>}
+then @{text \<open>a\<close>} can impersonate all @{text \<open>b\<close>} (take all of @{text \<open>b\<close>}'s "roles") where
+the @{text \<open>b\<close>}'s are specified by a given set of identities.\<close>
 definition Insider :: "[identity, identity set, identity \<Rightarrow> actor_state] \<Rightarrow> bool" 
 where "Insider a C as \<equiv> (tipping_point (as a) \<longrightarrow> (\<forall> b\<in>C. UasI a b))"
-
 definition Insider' :: "[actor \<Rightarrow> bool, identity, identity set, identity \<Rightarrow> actor_state] \<Rightarrow> bool" 
 where "Insider' P a C as \<equiv> (tipping_point (as a) \<longrightarrow> (\<forall> b\<in>C. UasI' P a b \<and> inj_on Actor C))"
-
+text \<open>The predicate @{text \<open>atI\<close>} -- mixfix syntax @{text \<open>@\<^bsub>G\<^esub>\<close>} -- expresses that an actor (identity) 
+      is at a certain location in an igraph.\<close>
 definition atI :: "[identity, igraph, location] \<Rightarrow> bool" ("_ @\<^bsub>(_)\<^esub> _" 50)
 where "a @\<^bsub>G\<^esub> l \<equiv> a \<in> set(agra G l)"
-
-text \<open>enables is the central definition of the behaviour as given by a policy
-that specifies what actions are allowed in a certain location for what actors \<close>
+text \<open>The enables predicate is the central definition of the behaviour as given by a policy
+that specifies what actions are allowed in a certain location for what actors.
+Policies specify the expected behaviour of actors of an infrastructure. 
+They are defined by the @{text \<open>enables\<close>} predicate:
+an actor @{text \<open>h\<close>} is enabled to perform an action @{text \<open>a\<close>} 
+in infrastructure @{text \<open>I\<close>}, at location @{text \<open>l\<close>}
+if there exists a pair @{text \<open>(p,e)\<close>} in the local policy of @{text \<open>l\<close>}
+(@{text \<open>delta I l\<close>} projects to the local policy) such that the action 
+@{text \<open>a\<close>} is a member of the action set @{text \<open>e\<close>} and the policy 
+predicate @{text \<open>p\<close>} holds for actor @{text \<open>h\<close>}.\<close>
 definition enables :: "[infrastructure, location, actor, action] \<Rightarrow> bool"
 where
 "enables I l a a' \<equiv>  (\<exists> (p,e) \<in> delta I (graphI I) l. a' \<in> e \<and> p a)"
+text \<open>For example, the @{text \<open>apolicy\<close>} pair @{text \<open>(\<lambda> x. True, {move})\<close>}
+specifies that all actors are enabled to perform action @{text \<open>move\<close>}.\<close>
 
-text \<open>behaviour is the good behaviour, i.e. everything allowed by policy \<close>
+text \<open>The behaviour is the good behaviour, i.e. everything allowed by the policy of 
+Infrastructure @{text \<open>I\<close>}.\<close>
 definition behaviour :: "infrastructure \<Rightarrow> (location * actor * action)set"
 where "behaviour I \<equiv> {(t,a,a'). enables I t a a'}"
 
-text \<open>misbehaviour is the complement of behaviour \<close>
+text \<open>The misbehaviour is the complement of behaviour of an Infrastructure @{text \<open>I\<close>}.\<close>
 definition misbehaviour :: "infrastructure \<Rightarrow> (location * actor * action)set"
   where "misbehaviour I \<equiv> -(behaviour I)"
 
-text \<open>basic lemmas for enable\<close>
-lemma not_enableI: "(\<forall> (p,e) \<in> delta I (graphI I) l. (~(h : e) | (~(p(a))))) 
-                     \<Longrightarrow> ~(enables I l a h)"
+text \<open>We prove some basic lemmas for the predicate @{text \<open>enable\<close>}.\<close>
+lemma not_enableI: "(\<forall> (p,e) \<in> delta I (graphI I) l. (\<not>(h : e) | (\<not>(p(a))))) 
+                     \<Longrightarrow> \<not>(enables I l a h)"
   by (simp add: enables_def, blast)
 
 lemma not_enableI2: "\<lbrakk>\<And> p e. (p,e) \<in> delta I (graphI I) l \<Longrightarrow>
-                 (~(t : e) |  (~(p(a)))) \<rbrakk> \<Longrightarrow> ~(enables I l a t)"
+                 (\<not>(t : e) |  (\<not>(p(a)))) \<rbrakk> \<Longrightarrow> \<not>(enables I l a t)"
  by (rule not_enableI, rule ballI, auto)
 
-lemma not_enableE: "\<lbrakk> ~(enables I l a t); (p,e) \<in> delta I (graphI I) l \<rbrakk>
-                 \<Longrightarrow> (~(t : e) |  (~(p(a))))"
+lemma not_enableE: "\<lbrakk> \<not>(enables I l a t); (p,e) \<in> delta I (graphI I) l \<rbrakk>
+                 \<Longrightarrow> (\<not>(t : e) |  (\<not>(p(a))))"
   by (simp add: enables_def, rule impI, force)
 
-lemma not_enableE2: "\<lbrakk> ~(enables I l a t); (p,e) \<in> delta I (graphI I) l;
-                     t : e \<rbrakk> \<Longrightarrow> (~(p(a)))"
+lemma not_enableE2: "\<lbrakk> \<not>(enables I l a t); (p,e) \<in> delta I (graphI I) l;
+                     t : e \<rbrakk> \<Longrightarrow> (\<not>(p(a)))"
   by (simp add: enables_def, force)
 
-text \<open>some constructions to deal with lists of actors in locations for 
-the semantics of action move\<close>
+subsection "State transition on infrastructures"
+text \<open>The state transition defines how actors may act on infrastructures through actions
+    within the boundaries of the policy. It is given as an inductive definition over the 
+    states which are infrastructures.  This state transition relation is dependent on actions but also on
+    enabledness and the current state of the infrastructure.
+
+    First we introduce some auxiliary functions dealing
+    with repetitions in lists and actors moving in an @{text \<open>igraph\<close>} and some 
+    constructions to deal with lists of actors in locations for the semantics of action 
+    @{text \<open>move\<close>}.\<close>
 primrec del :: "['a, 'a list] \<Rightarrow> 'a list"
 where 
 del_nil: "del a [] = []" |
@@ -168,7 +266,7 @@ where "move_graph_a n l l' g \<equiv> Lgraph (gra g)
                      else (agra g))(cgra g)(lgra g)"
 
 text \<open>State transition relation over infrastructures (the states) defining the 
-   semantics of actions in systems with humans and potentially insiders *)\<close>
+   semantics of actions in systems with humans and potentially insiders.\<close>
 inductive state_transition_in :: "[infrastructure, infrastructure] \<Rightarrow> bool" ("(_ \<rightarrow>\<^sub>n _)" 50)
 where
   move: "\<lbrakk> G = graphI I; a @\<^bsub>G\<^esub> l; l \<in> nodes G; l' \<in> nodes G;
@@ -196,10 +294,11 @@ where
                     (delta I) \<rbrakk>
          \<Longrightarrow> I \<rightarrow>\<^sub>n I'"
   
-text \<open>show that this infrastructure is a state as given in MC.thy\<close>
+text \<open>Note that the type infrastructure can now be instantiated to the axiomatic type class 
+      @{text\<open>state\<close>} which enables the use of the underlying Kripke structures and CTL.
+      We need to show that this infrastructure is a state as given in MC.thy\<close>
 instantiation "infrastructure" :: state
 begin
-
 definition 
    state_transition_infra_def: "(i \<rightarrow>\<^sub>i i') =  (i \<rightarrow>\<^sub>n (i' :: infrastructure))"
 
@@ -209,6 +308,7 @@ instance
 definition state_transition_in_refl ("(_ \<rightarrow>\<^sub>n* _)" 50)
 where "s \<rightarrow>\<^sub>n* s' \<equiv> ((s,s') \<in> {(x,y). state_transition_in x y}\<^sup>*)"
 
+text \<open>Lemmas about the auxiliary functions @{text \<open>del, jonce, nodup\<close>} are provided.\<close> 
 lemma del_del[rule_format]: "n \<in> set (del a S) \<longrightarrow> n \<in> set S"
   by (induct_tac S, auto)
     
@@ -250,7 +350,7 @@ lemma move_graph_eq: "move_graph_a a l l g = g"
   by (simp add: move_graph_a_def, case_tac g, force)
 
 text \<open>Some useful properties about the invariance of the nodes, the actors, and the policy 
-   with respect to the  state transition\<close> 
+   with respect to the  state transition are provided.\<close> 
 lemma delta_invariant: "\<forall> z z'. z \<rightarrow>\<^sub>n z' \<longrightarrow>  delta(z) = delta(z')"    
   by (clarify, erule state_transition_in.cases, simp+)
 
