MC.thy
@@ -8,37 +8,21 @@ imports Main
 begin
 
 subsection "Lemmas to support least and greatest fixpoints"
-definition monotone :: "('a set \<Rightarrow> 'a set) \<Rightarrow> bool"
-where "monotone \<tau> \<equiv> (\<forall> p q. p \<subseteq> q \<longrightarrow> \<tau> p \<subseteq> \<tau> q )"
-
-lemma monotoneE: "monotone \<tau> \<Longrightarrow> p \<subseteq> q \<Longrightarrow> \<tau> p \<subseteq> \<tau> q"
-by (simp add: monotone_def)
-
-lemma lfp1: "monotone \<tau> \<longrightarrow> (lfp \<tau> = \<Inter> {Z. \<tau> Z \<subseteq> Z})"
-by (simp add: monotone_def lfp_def)
-
-lemma gfp1: "monotone \<tau> \<longrightarrow> (gfp \<tau> = \<Union> {Z. Z \<subseteq> \<tau> Z})"
-by (simp add: monotone_def gfp_def)
-
-primrec power :: "['a \<Rightarrow> 'a, nat] \<Rightarrow> ('a \<Rightarrow> 'a)" ("(_ ^ _)" 40)
-where 
-power_zero: "(f ^ 0) = (\<lambda> x. x)" |
-power_suc: "(f ^ (Suc n)) = (f o (f ^ n))"
 
 lemma predtrans_empty: 
-  assumes "monotone \<tau>"
-  shows "\<forall> i. (\<tau> ^ i) ({}) \<subseteq> (\<tau> ^(i + 1))({})"
+  assumes "mono (\<tau> :: 'a set \<Rightarrow> 'a set)"
+  shows "\<forall> i. (\<tau> ^^ i) ({}) \<subseteq> (\<tau> ^^(i + 1))({})"
 proof (rule allI, induct_tac i)
-  show "(\<tau> ^ 0::nat) {} \<subseteq> (\<tau> ^ (0::nat) + (1::nat)) {}" by simp
-next show "\<And>(i::nat) n::nat. (\<tau> ^ n) {} \<subseteq> (\<tau> ^ n + (1::nat)) {} 
-      \<Longrightarrow> (\<tau> ^ Suc n) {} \<subseteq> (\<tau> ^ Suc n + (1::nat)) {}"
+  show "\<And>i::nat. (\<tau> ^^ (0::nat)) {} \<subseteq> (\<tau> ^^ ((0::nat) + (1::nat))) {}" 
+   by simp
+next show "\<And>(i::nat) n::nat. (\<tau> ^^ n) {} \<subseteq> (\<tau> ^^ (n + (1::nat))) {} 
+      \<Longrightarrow> (\<tau> ^^ Suc n) {} \<subseteq> (\<tau> ^^ (Suc n + (1::nat))) {}"
   proof -
     fix i n
-    assume a : " (\<tau> ^ n) {} \<subseteq> (\<tau> ^ n + (1::nat)) {}"
-    have "(\<tau> ((\<tau> ^ n) {})) \<subseteq> (\<tau> ((\<tau> ^ (n + (1 :: nat))) {}))" using assms
-      apply (rule monotoneE)
-      by (rule a)
-    thus "(\<tau> ^ Suc n) {} \<subseteq> (\<tau> ^ Suc n + (1::nat)) {}" by simp
+    assume a : " (\<tau> ^^ n) {} \<subseteq> (\<tau> ^^ (n + (1::nat))) {}"
+    have "(\<tau> ((\<tau> ^^ n) {})) \<subseteq> (\<tau> ((\<tau> ^^ (n + (1 :: nat))) {}))" using assms
+      using a monoE by blast
+    thus "(\<tau> ^^ Suc n) {} \<subseteq> (\<tau> ^^ (Suc n + (1::nat))) {}" by simp
   qed
 qed
 
@@ -50,126 +34,101 @@ by arith
 
 lemma infchain_outruns_all: 
   assumes "finite (UNIV :: 'a set)" 
-    and "\<forall>i :: nat. (\<tau> ^ i) ({}:: 'a set) \<subset> (\<tau> ^ i + (1 :: nat)) {}"
-  shows "\<forall>j :: nat. \<exists>i :: nat. j < card ((\<tau> ^ i) {})"
+    and "\<forall>i :: nat. ((\<tau> :: 'a set \<Rightarrow> 'a set)^^ i) ({}:: 'a set) \<subset> (\<tau> ^^ (i + (1 :: nat))) {}"
+  shows "\<forall>j :: nat. \<exists>i :: nat. j < card ((\<tau> ^^ i) {})"
 proof (rule allI, induct_tac j)
-  show "\<exists>i::nat. (0::nat) < card ((\<tau> ^ i) {})" using assms   
+  show "\<exists>i::nat. (0::nat) < card ((\<tau> ^^ i) {})" using assms   
     apply (drule_tac x = 0 in spec)
     apply (rule_tac x = 1 in exI)
     apply simp
-    apply (subgoal_tac "card {} = 0")
-    apply (erule subst)
-    apply (rule psubset_card_mono)
-    apply (rule_tac B = UNIV in finite_subset)
-    apply simp
-    apply assumption+
-      by simp
-  next show "\<And>(j::nat) n::nat. \<exists>i::nat. n < card ((\<tau> ^ i) {}) 
-             \<Longrightarrow> \<exists>i::nat. Suc n < card ((\<tau> ^ i) {})"
+    by (metis bot.not_eq_extremum card_gt_0_iff finite_subset subset_UNIV)
+next show "\<And>(j::nat) n::nat. \<exists>i::nat. n < card ((\<tau> ^^ i) {}) 
+             \<Longrightarrow> \<exists>i::nat. Suc n < card ((\<tau> ^^ i) {})"
     proof -
       fix j n
-      assume a: "\<exists>i::nat. n < card ((\<tau> ^ i) {})"
-      obtain i where "n < card ((\<tau> ^ (i :: nat)) {})" 
-        apply (rule exE)
-         apply (rule a)
-        by simp
-      thus "\<exists> i. Suc n < card ((\<tau> ^ i) {})" using assms
-        apply (rule_tac x = "i + 1" in exI)
-        apply (subgoal_tac "card((\<tau> ^ i) {}) < card((\<tau> ^ i + (1 :: nat)) {})")
-        apply arith
-        apply (rule psubset_card_mono)
-        apply (rule_tac B = UNIV in finite_subset)
-        apply simp
-        apply (rule assms)
-        by (erule spec)
+      assume a: "\<exists>i::nat. n < card ((\<tau> ^^ i) {})"
+      obtain i where "n < card ((\<tau> ^^ (i :: nat)) {})"
+        using a by blast 
+      thus "\<exists> i. Suc n < card ((\<tau> ^^ i) {})" using assms
+        by (meson finite_subset le_less_trans le_simps(3) psubset_card_mono subset_UNIV)
     qed
   qed
 
 lemma no_infinite_subset_chain: 
    assumes "finite (UNIV :: 'a set)"
-    and    "monotone (\<tau> :: ('a set \<Rightarrow> 'a set))"
-    and    "\<forall>i :: nat. ((\<tau> :: 'a set \<Rightarrow> 'a set) ^ i) {} \<subset> (\<tau> ^ i + (1 :: nat)) ({} :: 'a set)" 
+    and    "mono (\<tau> :: ('a set \<Rightarrow> 'a set))"
+    and    "\<forall>i :: nat. ((\<tau> :: 'a set \<Rightarrow> 'a set) ^^ i) {} \<subset> (\<tau> ^^ (i + (1 :: nat))) ({} :: 'a set)" 
   shows   "False"
 text \<open>Proof idea: since @{term "UNIV"} is finite, we have from @{text \<open>ex_card\<close>} that there is
     an n with @{term "card UNIV = n"}. Now, use @{text \<open>infchain_outruns_all\<close>} to show as 
     contradiction point that
-    @{term "\<exists> i :: nat. card UNIV < card ((\<tau> ^ i) {})"}. 
+    @{term "\<exists> i :: nat. card UNIV < card ((\<tau> ^^ i) {})"}. 
     Since all sets are subsets of @{term "UNIV"}, we also have 
-    @{term "card ((\<tau> ^ i) {}) \<le> card UNIV"}:
+    @{term "card ((\<tau> ^^ i) {}) \<le> card UNIV"}:
     Contradiction!, i.e. proof of False  \<close>
 proof -
-  have a: "\<forall> (j :: nat). (\<exists> (i :: nat). (j :: nat) < card((\<tau> ^ i)({} :: 'a set)))" using assms
-    apply (erule_tac \<tau> = \<tau> in infchain_outruns_all)
-    by assumption
+  have a: "\<forall> (j :: nat). (\<exists> (i :: nat). (j :: nat) < card((\<tau> ^^ i)({} :: 'a set)))" using assms
+    by (erule_tac \<tau> = \<tau> in infchain_outruns_all)
   hence b: "\<exists> (n :: nat). card(UNIV :: 'a set) = n" using assms
     by (erule_tac S = UNIV in ex_card)
   from this obtain n where c: "card(UNIV :: 'a set) = n" by (erule exE)
-  hence   d: "\<exists>i::nat. card UNIV < card ((\<tau> ^ i) {})" using a
-    apply (drule_tac x = "card UNIV" in spec)
-    by assumption
-  from this obtain i where e: "card (UNIV :: 'a set) < card ((\<tau> ^ i) {})"
+  hence   d: "\<exists>i::nat. card UNIV < card ((\<tau> ^^ i) {})" using a
+    by (drule_tac x = "card UNIV" in spec)
+  from this obtain i where e: "card (UNIV :: 'a set) < card ((\<tau> ^^ i) {})"
     by (erule exE)
-  hence f: "(card((\<tau> ^ i){})) \<le> (card (UNIV :: 'a set))" using assms
-    thm Finite_Set.card_mono
-      apply (rule_tac A = "((\<tau> ^ i){})" in Finite_Set.card_mono)
-      apply assumption
+  hence f: "(card((\<tau> ^^ i){})) \<le> (card (UNIV :: 'a set))" using assms
+    apply (erule_tac A = "((\<tau> ^^ i){})" in Finite_Set.card_mono)
     by (rule subset_UNIV)
   thus "False" using e
-    thm less_not_le
-    apply (erule_tac y = "card((\<tau> ^ i){})" in less_not_le)
-    by assumption
+    by (erule_tac y = "card((\<tau> ^^ i){})" in less_not_le)
 qed
 
 lemma finite_fixp: 
   assumes "finite(UNIV :: 'a set)" 
-      and "monotone (\<tau> :: ('a set \<Rightarrow> 'a set))"
-    shows "\<exists> i. (\<tau> ^ i) ({}) = (\<tau> ^(i + 1))({})"
+      and "mono (\<tau> :: ('a set \<Rightarrow> 'a set))"
+    shows "\<exists> i. (\<tau> ^^ i) ({}) = (\<tau> ^^(i + 1))({})"
 text \<open>Proof idea: 
 with @{text predtrans_empty} we know 
 
-@{term "\<forall> i. (\<tau> ^ i){} \<subseteq> (\<tau> ^(i + 1))({})"} (1).
+@{term "\<forall> i. (\<tau> ^^ i){} \<subseteq> (\<tau> ^^(i + 1))({})"} (1).
 
 If we can additionally show 
 
-@{term "\<exists> i.  (\<tau> ^ i)({}) \<supseteq> (\<tau> ^(i + 1))({})"} (2),
+@{term "\<exists> i.  (\<tau> ^^ i)({}) \<supseteq> (\<tau> ^^(i + 1))({})"} (2),
 
 we can get the goal together with equalityI 
 @{text "\<subseteq> + \<supseteq> \<longrightarrow> ="}. 
 To prove (1) we observe that 
-@{term "(\<tau> ^ i)({}) \<supseteq> (\<tau> ^(i + 1))({})"} 
+@{term "(\<tau> ^^ i)({}) \<supseteq> (\<tau> ^^(i + 1))({})"} 
 can be inferred from 
-@{term "\<not>((\<tau> ^ i)({}) \<subseteq> (\<tau> ^(i + 1))({}))"} 
+@{term "\<not>((\<tau> ^^ i)({}) \<subseteq> (\<tau> ^^(i + 1))({}))"} 
 and (1).
 Finally, the latter is solved directly by @{text \<open>no_infinite_subset_chain\<close>}.\<close>
 proof -
-  have a: "\<forall>i::nat. (\<tau> ^ i) ({}:: 'a set) \<subseteq> (\<tau> ^ i + (1::nat)) {}" 
-    thm predtrans_empty
-    apply(rule predtrans_empty)
-    by (rule assms(2))
-  hence b: "(\<exists> i :: nat. \<not>((\<tau> ^ i) {} \<subset> (\<tau> ^(i + 1)) {}))" using assms
-    apply (subgoal_tac "\<not> (\<forall> i :: nat. (\<tau> ^ i) {} \<subset> (\<tau> ^(i + 1)) {})")
-    apply blast
-    apply (rule notI)
-    apply (rule no_infinite_subset_chain)
-    by assumption
-  thus "\<exists> i. (\<tau> ^ i) ({}) = (\<tau> ^(i + 1))({})" using a
+  have a: "\<forall>i::nat. (\<tau> ^^ i) ({}:: 'a set) \<subseteq> (\<tau> ^^ (i + (1::nat))) {}" 
+    by(rule predtrans_empty, rule assms(2))
+  have a3: "\<not> (\<forall> i :: nat. (\<tau> ^^ i) {} \<subset> (\<tau> ^^(i + 1)) {})" 
+    by (rule notI, rule no_infinite_subset_chain, (rule assms)+)
+  hence b: "(\<exists> i :: nat. \<not>((\<tau> ^^ i) {} \<subset> (\<tau> ^^(i + 1)) {}))" using assms a3
+    by blast
+  thus "\<exists> i. (\<tau> ^^ i) ({}) = (\<tau> ^^(i + 1))({})" using a
     by blast
 qed
 
 lemma predtrans_UNIV: 
-  assumes "monotone \<tau>"
-  shows "\<forall> i. (\<tau> ^ i) (UNIV) \<supseteq> (\<tau> ^(i + 1))(UNIV)"
+  assumes "mono (\<tau> :: ('a set \<Rightarrow> 'a set))"
+  shows "\<forall> i. (\<tau> ^^ i) (UNIV) \<supseteq> (\<tau> ^^(i + 1))(UNIV)"
 proof (rule allI, induct_tac i)
-  show "(\<tau> ^ (0::nat) + (1::nat)) UNIV \<subseteq> (\<tau> ^ 0::nat) UNIV" by simp
+  show "(\<tau> ^^ ((0::nat) + (1::nat))) UNIV \<subseteq> (\<tau> ^^ (0::nat)) UNIV" 
+    by simp
 next show "\<And>(i::nat) n::nat.
-       (\<tau> ^ n + (1::nat)) UNIV \<subseteq> (\<tau> ^ n) UNIV \<Longrightarrow> (\<tau> ^ Suc n + (1::nat)) UNIV \<subseteq> (\<tau> ^ Suc n) UNIV"
+       (\<tau> ^^ (n + (1::nat))) UNIV \<subseteq> (\<tau> ^^ n) UNIV \<Longrightarrow> (\<tau> ^^ (Suc n + (1::nat))) UNIV \<subseteq> (\<tau> ^^ Suc n) UNIV"
   proof -
     fix i n
-    assume a: "(\<tau> ^ n + (1::nat)) UNIV \<subseteq> (\<tau> ^ n) UNIV"
-    have "(\<tau> ((\<tau> ^ n) UNIV)) \<supseteq> (\<tau> ((\<tau> ^ (n + (1 :: nat))) UNIV))" using assms
-      apply (rule monotoneE)
-      by (rule a)
-    thus "(\<tau> ^ Suc n + (1::nat)) UNIV \<subseteq> (\<tau> ^ Suc n) UNIV" by simp
+    assume a: "(\<tau> ^^ (n + (1::nat))) UNIV \<subseteq> (\<tau> ^^ n) UNIV"
+    have "(\<tau> ((\<tau> ^^ n) UNIV)) \<supseteq> (\<tau> ((\<tau> ^^ (n + (1 :: nat))) UNIV))" using assms a
+      by (rule monoE)
+    thus "(\<tau> ^^ (Suc n + (1::nat))) UNIV \<subseteq> (\<tau> ^^ Suc n) UNIV" by simp
    qed
  qed
 
@@ -177,138 +136,97 @@ lemma Suc_less_le: "x < (y - n) \<Longrightarrow> x \<le> (y - (Suc n))"
  by simp
 
 lemma card_univ_subtract: 
-  assumes "finite (UNIV :: 'a set)" and  "monotone (\<tau> :: 'a set \<Rightarrow> 'a set)"
-     and  "(\<forall>i :: nat. ((\<tau> :: 'a set \<Rightarrow> 'a set) ^ i + (1 :: nat)) (UNIV :: 'a set) \<subset> (\<tau> ^ i) UNIV)"
-   shows "(\<forall> i :: nat. card((\<tau> ^ i) (UNIV ::'a set)) \<le> (card (UNIV :: 'a set)) - i)"
+  assumes "finite (UNIV :: 'a set)" and  "mono (\<tau> :: ('a set \<Rightarrow> 'a set))"
+     and  "(\<forall>i :: nat. ((\<tau> :: 'a set \<Rightarrow> 'a set) ^^ (i + (1 :: nat)))(UNIV :: 'a set) \<subset> (\<tau> ^^ i) UNIV)"
+   shows "(\<forall> i :: nat. card((\<tau> ^^ i) (UNIV ::'a set)) \<le> (card (UNIV :: 'a set)) - i)"
 proof (rule allI, induct_tac i) 
-  show "card ((\<tau> ^ 0::nat) UNIV) \<le> card (UNIV :: 'a set) - (0::nat)" using assms
+  show "card ((\<tau> ^^ (0::nat)) UNIV) \<le> card (UNIV :: 'a set) - (0::nat)" using assms
     by (simp)
 next show "\<And>(i::nat) n::nat.
-       card ((\<tau> ^ n) (UNIV :: 'a set)) \<le> card (UNIV :: 'a set) - n \<Longrightarrow>
-       card ((\<tau> ^ Suc n) (UNIV :: 'a set)) \<le> card (UNIV :: 'a set) - Suc n" using assms
+       card ((\<tau> ^^ n) (UNIV :: 'a set)) \<le> card (UNIV :: 'a set) - n \<Longrightarrow>
+       card ((\<tau> ^^ Suc n) (UNIV :: 'a set)) \<le> card (UNIV :: 'a set) - Suc n" using assms
   proof -
     fix i n
-    assume a: "card ((\<tau> ^ n) (UNIV :: 'a set)) \<le> card (UNIV :: 'a set) - n"
-    have b: "(\<tau> ^ n + (1::nat)) (UNIV :: 'a set) \<subset> (\<tau> ^ n) UNIV" using assms
+    assume a: "card ((\<tau> ^^ n) (UNIV :: 'a set)) \<le> card (UNIV :: 'a set) - n"
+    have b: "(\<tau> ^^ (n + (1::nat)))(UNIV :: 'a set) \<subset> (\<tau> ^^ n) UNIV" using assms
       by (erule_tac x = n in spec)
-    have "card((\<tau> ^ n + (1 :: nat)) (UNIV :: 'a set)) < card((\<tau> ^ n) (UNIV :: 'a set))" 
-      apply (rule psubset_card_mono)
-      apply (rule finite_subset) 
-      apply (rule subset_UNIV)
-       apply (rule assms(1))
-      by (rule b)
-    thus "card ((\<tau> ^ Suc n) (UNIV :: 'a set)) \<le> card (UNIV :: 'a set) - Suc n" using a
+    have "card((\<tau> ^^ (n + (1 :: nat)))(UNIV :: 'a set)) < card((\<tau> ^^ n) (UNIV :: 'a set))"       
+      by (rule psubset_card_mono, rule finite_subset, rule subset_UNIV, rule assms(1), rule b)
+    thus "card ((\<tau> ^^ Suc n) (UNIV :: 'a set)) \<le> card (UNIV :: 'a set) - Suc n" using a
       by simp
     qed
   qed
 
 lemma card_UNIV_tau_i_below_zero: 
-  assumes "finite (UNIV :: 'a set)" and "monotone (\<tau> :: 'a set \<Rightarrow> 'a set)"
-   and  "(\<forall>i :: nat. ((\<tau> :: 'a set \<Rightarrow> 'a set) ^ i + (1 :: nat)) (UNIV :: 'a set) \<subset> (\<tau> ^ i) UNIV)"
- shows "card((\<tau> ^ (card (UNIV ::'a set))) (UNIV ::'a set)) \<le> 0"
+  assumes "finite (UNIV :: 'a set)" and "mono (\<tau> :: ('a set \<Rightarrow> 'a set))"
+   and  "(\<forall>i :: nat. ((\<tau> :: ('a set \<Rightarrow> 'a set)) ^^ (i + (1 :: nat)))(UNIV :: 'a set) \<subset> (\<tau> ^^ i) UNIV)"
+ shows "card((\<tau> ^^ (card (UNIV ::'a set))) (UNIV ::'a set)) \<le> 0"
 proof -
-  have "(\<forall> i :: nat. card((\<tau> ^ i) (UNIV ::'a set)) \<le> (card (UNIV :: 'a set)) - i)" using assms
+  have "(\<forall> i :: nat. card((\<tau> ^^ i) (UNIV ::'a set)) \<le> (card (UNIV :: 'a set)) - i)" using assms
     by (rule card_univ_subtract)
-  thus "card((\<tau> ^ (card (UNIV ::'a set))) (UNIV ::'a set)) \<le> 0"
-   apply (drule_tac x = "card (UNIV ::'a set)" in spec)
-    by simp
+  thus "card((\<tau> ^^ (card (UNIV ::'a set))) (UNIV ::'a set)) \<le> 0"
+   by (drule_tac x = "card (UNIV ::'a set)" in spec, simp)
 qed
 
 lemma finite_card_zero_empty: "\<lbrakk> finite S; card S \<le> 0\<rbrakk> \<Longrightarrow> S = {}"
 by simp
 
 lemma UNIV_tau_i_is_empty:
-  assumes "finite (UNIV :: 'a set)" and "monotone (\<tau> :: 'a set \<Rightarrow> 'a set)"
-    and   "(\<forall>i :: nat. ((\<tau> :: 'a set \<Rightarrow> 'a set) ^ i + (1 :: nat)) (UNIV :: 'a set) \<subset> (\<tau> ^ i) UNIV)"
-  shows "(\<tau> ^ (card (UNIV ::'a set))) (UNIV ::'a set) = {}"
-proof - 
-  have "card ((\<tau> ^ card (UNIV ::'a set)) UNIV) \<le> (0::nat)" using assms
-    apply (rule card_UNIV_tau_i_below_zero) 
-    .
-  thus "(\<tau> ^ (card (UNIV ::'a set))) (UNIV ::'a set) = {}" using assms
-    apply (rule_tac S = "(\<tau> ^ (card (UNIV ::'a set))) (UNIV ::'a set)" in finite_card_zero_empty)
-    apply (rule finite_subset)
-    apply (rule subset_UNIV)
-    .
-qed
+  assumes "finite (UNIV :: 'a set)" and "mono (\<tau> :: ('a set \<Rightarrow> 'a set))"
+    and   "(\<forall>i :: nat. ((\<tau> :: 'a set \<Rightarrow> 'a set) ^^ (i + (1 :: nat)))(UNIV :: 'a set) \<subset> (\<tau> ^^ i) UNIV)"
+  shows "(\<tau> ^^ (card (UNIV ::'a set))) (UNIV ::'a set) = {}"
+  by (meson assms card_UNIV_tau_i_below_zero finite_card_zero_empty finite_subset subset_UNIV)
 
 lemma down_chain_reaches_empty:
-  assumes "finite (UNIV :: 'a set)" and "monotone (\<tau> :: 'a set \<Rightarrow> 'a set)"
-   and "(\<forall>i :: nat. ((\<tau> :: 'a set \<Rightarrow> 'a set) ^ i + (1 :: nat)) UNIV \<subset> (\<tau> ^ i) UNIV)"
- shows "\<exists> (j :: nat). (\<tau> ^ j) UNIV = {}"
-proof -
-  have "(\<tau> ^ ((card (UNIV :: 'a set)))) UNIV = {}" using assms
-    apply (rule UNIV_tau_i_is_empty)
-    .
-  thus "\<exists> (j :: nat). (\<tau> ^ j) UNIV = {}" 
-    by (rule exI)
-qed
+  assumes "finite (UNIV :: 'a set)" and "mono (\<tau> :: 'a set \<Rightarrow> 'a set)"
+   and "(\<forall>i :: nat. ((\<tau> :: 'a set \<Rightarrow> 'a set) ^^ (i + (1 :: nat))) UNIV \<subset> (\<tau> ^^ i) UNIV)"
+ shows "\<exists> (j :: nat). (\<tau> ^^ j) UNIV = {}"
+  using UNIV_tau_i_is_empty assms by blast
 
 lemma no_infinite_subset_chain2: 
-  assumes "finite (UNIV :: 'a set)" and "monotone (\<tau> :: ('a set \<Rightarrow> 'a set))"
-      and "\<forall>i :: nat. (\<tau> ^ i) UNIV \<supset> (\<tau> ^ i + (1 :: nat)) UNIV"
+  assumes "finite (UNIV :: 'a set)" and "mono (\<tau> :: ('a set \<Rightarrow> 'a set))"
+      and "\<forall>i :: nat. (\<tau> ^^ i) UNIV \<supset> (\<tau> ^^ (i + (1 :: nat))) UNIV"
   shows "False"
 proof -
-  have "\<exists> j :: nat. (\<tau> ^ j) UNIV = {}" using assms
-    apply (rule down_chain_reaches_empty)
-    .
-  from this obtain j where a: "(\<tau> ^ j) UNIV = {}" by (erule exE)
-  have "(\<tau> ^ j + (1::nat)) UNIV \<subset> (\<tau> ^ j) UNIV" using assms
+  have "\<exists> j :: nat. (\<tau> ^^ j) UNIV = {}" using assms
+    by (rule down_chain_reaches_empty)
+  from this obtain j where a: "(\<tau> ^^ j) UNIV = {}" by (erule exE)
+  have "(\<tau> ^^ (j + (1::nat))) UNIV \<subset> (\<tau> ^^ j) UNIV" using assms
     by (erule_tac x = j in spec)
   thus False using a by simp 
 qed
 
 lemma finite_fixp2: 
-  assumes "finite(UNIV :: 'a set)" and "monotone (\<tau> :: ('a set \<Rightarrow> 'a set))"
-  shows "\<exists> i. (\<tau> ^ i) UNIV = (\<tau> ^(i + 1)) UNIV"
+  assumes "finite(UNIV :: 'a set)" and "mono (\<tau> :: ('a set \<Rightarrow> 'a set))"
+  shows "\<exists> i. (\<tau> ^^ i) UNIV = (\<tau> ^^(i + 1)) UNIV"
 proof -
-  have "\<forall>i::nat. (\<tau> ^ i + (1::nat)) UNIV \<subseteq> (\<tau> ^ i) UNIV" 
-    apply (rule predtrans_UNIV) using assms
-    by (simp add: assms(2))
-  moreover have "\<exists>i::nat. \<not> (\<tau> ^ i + (1::nat)) UNIV \<subset> (\<tau> ^ i) UNIV" using assms
+  have "\<forall>i::nat. (\<tau> ^^ (i + (1::nat))) UNIV \<subseteq> (\<tau> ^^ i) UNIV" 
+    by (rule predtrans_UNIV , simp add: assms(2))  
+  moreover have "\<exists>i::nat. \<not> (\<tau> ^^ (i + (1::nat))) UNIV \<subset> (\<tau> ^^ i) UNIV" using assms
   proof -
-    have "\<not> (\<forall> i :: nat. (\<tau> ^ i) UNIV \<supset> (\<tau> ^(i + 1)) UNIV)" 
-      apply (rule notI) 
-      apply (rule no_infinite_subset_chain2) using assms
-      .
-    thus "\<exists>i::nat. \<not> (\<tau> ^ i + (1::nat)) UNIV \<subset> (\<tau> ^ i) UNIV" by blast
+    have "\<not> (\<forall> i :: nat. (\<tau> ^^ i) UNIV \<supset> (\<tau> ^^(i + 1)) UNIV)"
+      using assms(1) assms(2) no_infinite_subset_chain2 by blast 
+    thus "\<exists>i::nat. \<not> (\<tau> ^^ (i + (1::nat))) UNIV \<subset> (\<tau> ^^ i) UNIV" by blast
   qed
-  ultimately show "\<exists> i. (\<tau> ^ i) UNIV = (\<tau> ^(i + 1)) UNIV" 
+  ultimately show "\<exists> i. (\<tau> ^^ i) UNIV = (\<tau> ^^(i + 1)) UNIV" 
     by blast
 qed
 
-lemma mono_monotone: "mono (\<tau> :: ('a set \<Rightarrow> 'a set)) \<Longrightarrow> monotone \<tau>"
-by (simp add: monotone_def mono_def)
-
-lemma monotone_mono: "monotone (\<tau> :: ('a set \<Rightarrow> 'a set)) \<Longrightarrow> mono \<tau>"
-by (simp add: monotone_def mono_def)
-
-lemma power_power: "((\<tau> :: ('a set \<Rightarrow> 'a set)) ^^ n) = ((\<tau> :: ('a set \<Rightarrow> 'a set)) ^ n)"
-proof (induct_tac n)
-  show "\<tau> ^^ (0::nat) = (\<tau> ^ 0::nat)" by (simp add: id_def)
-next show "\<And>n::nat. \<tau> ^^ n = (\<tau> ^ n) \<Longrightarrow> \<tau> ^^ Suc n = (\<tau> ^ Suc n)"
-    by simp
-qed
-
-lemma lfp_Kleene_iter_set: "monotone (f :: ('a set \<Rightarrow> 'a set)) \<Longrightarrow>
-   (f ^ Suc(n)) {} = (f ^ n) {} \<Longrightarrow> lfp f  = (f ^ n){}"
-by (simp add: monotone_mono lfp_Kleene_iter power_power)
-
 lemma lfp_loop: 
-  assumes "finite (UNIV :: 'b set)" and "monotone (\<tau> :: ('b set \<Rightarrow> 'b set))"
-  shows "\<exists> n . lfp \<tau>  = (\<tau> ^ n) {}"
+  assumes "finite (UNIV :: 'b set)" and "mono (\<tau> :: ('b set \<Rightarrow> 'b set))"
+  shows "\<exists> n . lfp \<tau>  = (\<tau> ^^ n) {}"
 proof -
-  have "\<exists>i::nat. (\<tau> ^ i) {} = (\<tau> ^ i + (1::nat)) {}"  using assms
+  have "\<exists>i::nat. (\<tau> ^^ i) {} = (\<tau> ^^ (i + (1::nat))) {}"  using assms
     by (rule finite_fixp)
-  from this obtain i where " (\<tau> ^ i) {} = (\<tau> ^ i + (1::nat)) {}"
+  from this obtain i where " (\<tau> ^^ i) {} = (\<tau> ^^ (i + (1::nat))) {}"
     by (erule exE)
-  hence "(\<tau> ^ i) {} = (\<tau> ^ Suc i) {}"
+  hence "(\<tau> ^^ i) {} = (\<tau> ^^ Suc i) {}"
     by simp
-  hence "(\<tau> ^ Suc i) {} = (\<tau> ^ i) {}"
+  hence "(\<tau> ^^ Suc i) {} = (\<tau> ^^ i) {}"
     by (rule sym)
-  hence "lfp \<tau> = (\<tau> ^ i) {}"
-     by (simp add: assms(2) lfp_Kleene_iter_set)
-   thus   "\<exists> n . lfp \<tau>  = (\<tau> ^ n) {}" 
+  hence "lfp \<tau> = (\<tau> ^^ i) {}"
+     by (simp add: assms(2) lfp_Kleene_iter)
+   thus   "\<exists> n . lfp \<tau>  = (\<tau> ^^ n) {}" 
    by (rule exI) 
 qed
 
@@ -336,37 +254,24 @@ next
     using Kleene_iter_gpfp[OF assms(1)] gfp_unfold[OF assms(1)] by simp
 qed
 
+
+(* same as gfp_Kleen_iter just instantiated to UNIV = top *)
 lemma gfp_Kleene_iter_set: 
-  assumes "monotone (f :: ('a set \<Rightarrow> 'a set))"
-      and "(f ^ Suc(n)) UNIV = (f ^ n) UNIV"
-    shows "gfp f  = (f ^ n) UNIV"
-proof -
-  have a: "mono f" using assms
-    by (erule_tac \<tau> = f in monotone_mono)
-  hence b: "(f ^^ Suc (n)) UNIV = (f ^^ n) UNIV" using assms
-    by (simp add: power_power)
-  hence c: "gfp f = (f ^^ (n))(UNIV :: 'a set)" using assms a
-    thm gfp_Kleene_iter
-    apply (erule_tac f = f and k = n in gfp_Kleene_iter)
-    .
-  thus "gfp f = (f ^ (n))(UNIV :: 'a set)" using assms a
-    by (simp add: power_power)
-qed    
-    
+  assumes "mono (f :: ('a set \<Rightarrow> 'a set))"
+      and "(f ^^ Suc(n)) UNIV = (f ^^ n) UNIV"
+    shows "gfp f  = (f ^^ n) UNIV"
+  by (rule  Nat.gfp_Kleene_iter, rule assms, rule assms)
+
 lemma gfp_loop: 
   assumes "finite (UNIV :: 'b set)"
-   and "monotone (\<tau> :: ('b set \<Rightarrow> 'b set))"
-    shows "\<exists> n . gfp \<tau>  = (\<tau> ^ n)(UNIV :: 'b set)"
+   and "mono (\<tau> :: ('b set \<Rightarrow> 'b set))"
+    shows "\<exists> n . gfp \<tau>  = (\<tau> ^^ n)(UNIV :: 'b set)"
 proof -
-  have " \<exists>i::nat. (\<tau> ^ i)(UNIV :: 'b set) = (\<tau> ^ i + (1::nat)) UNIV" using assms
+  have " \<exists>i::nat. (\<tau> ^^ i)(UNIV :: 'b set) = (\<tau> ^^ (i + (1::nat))) UNIV" using assms
     by (rule finite_fixp2)
-  from this obtain i where "(\<tau> ^ i)(UNIV :: 'b set) = (\<tau> ^ i + (1::nat)) UNIV" by (erule exE)
-  thus "\<exists> n . gfp \<tau>  = (\<tau> ^ n)(UNIV :: 'b set)" using assms
-    apply (rule_tac x = i in exI)
-    apply (rule gfp_Kleene_iter_set) 
-    apply assumption
-    apply (rule sym)
-    by simp
+  from this obtain i where "(\<tau> ^^ i)(UNIV :: 'b set) = (\<tau> ^^ (i + (1::nat))) UNIV" by (erule exE)
+  thus "\<exists> n . gfp \<tau>  = (\<tau> ^^ n)(UNIV :: 'b set)" using assms
+    by (metis Suc_eq_plus1 gfp_Kleene_iter_set)
 qed
 
 subsection \<open>Generic type of state with state transition and CTL operators\<close>
@@ -375,7 +280,7 @@ text \<open>The system states and their transition relation are defined as a cla
 syntactic infix notation @{text \<open>I \<rightarrow>\<^sub>i I'\<close>} to denote that system state @{text \<open>I\<close>} and @{text \<open>I’\<close>} 
 are in this relation over an arbitrary (polymorphic) type @{text \<open>'a\<close>}.\<close>
 class state =
-  fixes state_transition :: "['a :: type, 'a] \<Rightarrow> bool"  ("(_ \<rightarrow>\<^sub>i _)" 50)
+  fixes state_transition :: "['a :: type, 'a] \<Rightarrow> bool"  (infixr "\<rightarrow>\<^sub>i" 50)
 
 text \<open>The above class definition lifts Kripke structures and CTL to a general level. 
 The definition of the inductive relation is given by a set of specific rules which are, 
@@ -415,7 +320,7 @@ imply f.\<close>
 definition check ("_ \<turnstile> _" 50)
  where "M \<turnstile> f \<equiv> (init M) \<subseteq> {s \<in> (states M). s \<in> f }"
 
-definition state_transition_refl ("(_ \<rightarrow>\<^sub>i* _)" 50)
+definition state_transition_refl (infixr "\<rightarrow>\<^sub>i*" 50)
 where "s \<rightarrow>\<^sub>i* s' \<equiv> ((s,s') \<in> {(x,y). state_transition x y}\<^sup>*)"
   
 subsection \<open>Lemmas for CTL operators\<close>
@@ -425,10 +330,7 @@ lemma EF_lem0: "(x \<in> EF f) = (x \<in> f \<union> EX' (lfp (\<lambda>Z :: ('a
 proof -
   have "lfp (\<lambda>Z :: ('a :: state) set. f \<union> EX' Z) = 
                     f \<union> (EX' (lfp (\<lambda>Z :: 'a set. f \<union> EX' Z)))"
-    apply (rule def_lfp_unfold)
-    apply (rule reflexive)
-    apply (unfold mono_def EX'_def)
-    by auto
+    by (rule def_lfp_unfold, rule reflexive, unfold mono_def EX'_def, auto)
   thus "(x \<in> EF (f :: ('a :: state) set)) = (x \<in> f \<union> EX' (lfp (\<lambda>Z :: ('a :: state) set. f \<union> EX' Z)))"
     by (simp add: EF_def) 
 qed
@@ -436,18 +338,15 @@ qed
 lemma EF_lem00: "(EF f) = (f \<union> EX' (lfp (\<lambda> Z :: ('a :: state) set. f \<union> EX' Z)))"
 proof (rule equalityI)
   show "EF f \<subseteq> f \<union> EX' (lfp (\<lambda>Z::'a set. f \<union> EX' Z))"
-   apply (rule subsetI)
-   by (simp add: EF_lem0)
+   by (rule subsetI, simp add: EF_lem0)
   next show "f \<union> EX' (lfp (\<lambda>Z::'a set. f \<union> EX' Z)) \<subseteq> EF f"
-   apply (rule subsetI)
-   by (simp add: EF_lem0)
+   by (rule subsetI, simp add: EF_lem0)
  qed
 
 lemma EF_lem000: "(EF f) = (f \<union> EX' (EF f))"
 proof (subst EF_lem00)
   show "f \<union> EX' (lfp (\<lambda>Z::'a set. f \<union> EX' Z)) = f \<union> EX' (EF f)"
-    apply (fold EF_def)  
-    by (rule refl)
+    by (fold EF_def, rule refl)
 qed
 
 lemma EF_lem1: "x \<in> f \<or> x \<in> (EX' (EF f)) \<Longrightarrow> x \<in> EF f"
@@ -457,14 +356,10 @@ proof (simp add: EF_def)
   proof -
     have b: "lfp (\<lambda>Z :: ('a :: state) set. f \<union> EX' Z) =
                     f \<union> (EX' (lfp (\<lambda>Z :: ('a :: state) set. f \<union> EX' Z)))"
-      apply (rule def_lfp_unfold)
-      apply (rule reflexive)
-      apply (unfold mono_def EX'_def)
-      by auto
+      by (rule def_lfp_unfold, rule reflexive, unfold mono_def EX'_def, auto)
     thus "x \<in> lfp (\<lambda>Z::'a set. f \<union> EX' Z)" using a
-     apply (subst b)
-     by blast
- qed
+      by (subst b, blast)
+  qed   
 qed
 
 lemma EF_lem2b: 
@@ -472,15 +367,13 @@ lemma EF_lem2b:
    shows "x \<in> EF f"
 proof (rule EF_lem1)
   show "x \<in> f \<or> x \<in> EX' (EF f)" 
-    apply (rule disjI2)
-    by (rule assms)
+    by (rule disjI2, rule assms)
 qed
 
 lemma EF_lem2a: assumes "x \<in> f" shows "x \<in> EF f"
 proof (rule EF_lem1)
   show "x \<in> f \<or> x \<in> EX' (EF f)"
-    apply (rule disjI1)
-    by (rule assms)
+    by (rule disjI1, rule assms)
 qed
 
 lemma EF_lem2c: assumes "x \<notin> f" shows "x \<in> EF (- f)"
@@ -496,20 +389,14 @@ proof -
   have "x \<in> f \<Longrightarrow> x \<in> EF f" 
     by (erule EF_lem2a)
   thus "x \<notin> f" using assms
-    thm contrapos_nn
     apply (erule_tac P = "x \<in> f" in contrapos_nn)
-    apply (erule meta_mp)
-    .
+    by (erule meta_mp)
 qed
 
 lemma EF_lem3b: assumes "x \<in> EX' (f \<union> EX' (EF f))" shows "x \<in> (EF f)"
 proof (simp add: EF_lem0)
-  show "x \<in> f \<or> x \<in> EX' (lfp (\<lambda>Z::'a set. f \<union> EX' Z))" 
-   apply (rule disjI2)
-   apply (fold EF_def)
-   apply (subst EF_lem00)
-   apply (fold EF_def)
-   by (rule assms)
+  show "x \<in> f \<or> x \<in> EX' (lfp (\<lambda>Z::'a set. f \<union> EX' Z))"
+    by (metis EF_def EF_lem00 assms) 
 qed
 
 lemma EX_lem0l: "x \<in> (EX' f) \<Longrightarrow> x \<in> (EX' (f \<union> g))"
@@ -526,40 +413,30 @@ qed
 
 lemma EX_step: assumes "x  \<rightarrow>\<^sub>i y" and "y \<in> f" shows "x \<in> EX' f"
 proof (unfold EX'_def)
-  show " x \<in> {s::'a. \<exists>f0::'a\<in>f. s \<rightarrow>\<^sub>i f0}" 
-    apply simp
-    apply (rule_tac x = y in bexI)
-    by (rule assms)+
+  show " x \<in> {s::'a. \<exists>f0::'a\<in>f. s \<rightarrow>\<^sub>i f0}"
+    using assms(1) assms(2) by blast 
 qed
 
 lemma EF_E[rule_format]: "\<forall> f. x \<in> (EF (f :: ('a :: state) set)) \<longrightarrow> x \<in> (f \<union> EX' (EF f))"
 proof -
   have a: "\<And>f::'a set. EF (f :: ('a :: state) set) = f \<union> EX' (EF f)"
     by (rule EF_lem000)
-  thus "(\<forall> f. x \<in> EF (f :: ('a :: state) set) \<longrightarrow> x \<in> f \<union> EX' (EF f))" 
-    apply (rule_tac P = "(\<lambda> f. x \<in> EF (f :: ('a :: state) set) \<longrightarrow> x \<in> f \<union> EX' (EF f))" in allI)
-    apply (subst a) 
-    apply (rule impI)
-    by assumption
+  thus "(\<forall> f. x \<in> EF (f :: ('a :: state) set) \<longrightarrow> x \<in> f \<union> EX' (EF f))"
+    by auto 
 qed
 
 lemma EF_step: assumes "x  \<rightarrow>\<^sub>i y" and "y \<in> f" shows "x \<in> EF f"
 proof (rule EF_lem3b)
-  show "x \<in> EX' (f \<union> EX' (EF f))" 
-    apply (rule EX_step)
-    apply (rule assms(1))
-    by (simp add: assms(2))
+  show "x \<in> EX' (f \<union> EX' (EF f))"
+    using EX_step assms(1) assms(2) by blast 
 qed
 
 lemma EF_step_step: assumes "x  \<rightarrow>\<^sub>i y" and "y \<in> EF f" shows  "x \<in> EF f"
 proof -
   have "y \<in> f \<union> EX' (EF f)"
-    apply (rule EF_E)
-    by (rule assms(2))
+    by (rule EF_E, rule assms(2))
   thus "x \<in> EF f"
-    apply (rule_tac x = x and f = f in EF_lem3b)
-    apply (rule EX_step)
-    by (rule assms)
+    using EF_lem3b EX_step assms(1) by blast
 qed
 
 lemma EF_step_star: "\<lbrakk> x  \<rightarrow>\<^sub>i* y; y \<in> f \<rbrakk> \<Longrightarrow> x \<in> EF f"
@@ -568,29 +445,24 @@ proof (simp add: state_transition_refl_def)
   proof (erule converse_rtrancl_induct)
     show "y \<in> f \<Longrightarrow> y \<in> EF f" 
       by (erule EF_lem2a)
-    next show "\<And>(ya::'a) z::'a. y \<in> f \<Longrightarrow>
-                 (ya, z) \<in> {(x::'a, y::'a). x \<rightarrow>\<^sub>i y} \<Longrightarrow>
-                 (z, y) \<in> {(x::'a, y::'a). x \<rightarrow>\<^sub>i y}\<^sup>* \<Longrightarrow> z \<in> EF f \<Longrightarrow> ya \<in> EF f"
-        apply (clarify)
-        apply (erule EF_step_step)
-        by assumption
+    next show "\<And>ya z::'a. y \<in> f \<Longrightarrow>
+                 (ya, z) \<in> {(x,y). x \<rightarrow>\<^sub>i y} \<Longrightarrow>
+                 (z, y) \<in> {(x,y). x \<rightarrow>\<^sub>i y}\<^sup>* \<Longrightarrow> z \<in> EF f \<Longrightarrow> ya \<in> EF f"
+        by (simp add: EF_step_step)
     qed
   qed
 
 lemma EF_induct_prep: 
   assumes "(a::'a::state) \<in> lfp (\<lambda> Z. (f::'a::state set) \<union> EX' Z)"
-       and "mono  (\<lambda> Z. (f::'a::state set) \<union> EX' Z)"
-     shows "(\<And>x::'a::state.
+  and "mono  (\<lambda> Z. (f::'a::state set) \<union> EX' Z)"
+  shows "(\<And>x::'a::state.
      x \<in> ((\<lambda> Z. (f::'a::state set) \<union> EX' Z)(lfp (\<lambda> Z. (f::'a::state set) \<union> EX' Z) \<inter> {x::'a::state. (P::'a::state \<Rightarrow> bool) x})) \<Longrightarrow> P x) \<Longrightarrow>
       P a"
 proof -
   show "(\<And>x::'a::state.
      x \<in> ((\<lambda> Z. (f::'a::state set) \<union> EX' Z)(lfp (\<lambda> Z. (f::'a::state set) \<union> EX' Z) \<inter> {x::'a::state. (P::'a::state \<Rightarrow> bool) x})) \<Longrightarrow> P x) \<Longrightarrow>
       P a"
-    apply (rule_tac A = "EF f" in def_lfp_induct_set)
-    apply (rule EF_def)
-    apply (rule assms(2))
-    by (simp add: EF_def assms)+
+    by (rule_tac A = "EF f" in def_lfp_induct_set, rule EF_def, rule assms(2), (simp add: EF_def assms)+)
 qed
 
 lemma EF_induct: "(a::'a::state) \<in> EF (f :: 'a :: state set) \<Longrightarrow>
@@ -602,52 +474,30 @@ proof (simp add: EF_def)
   show "a \<in> lfp (\<lambda>Z::'a set. f \<union> EX' Z) \<Longrightarrow>
     mono (\<lambda>Z::'a set. f \<union> EX' Z) \<Longrightarrow>
     (\<And>x::'a. x \<in> f \<or> x \<in> EX' (lfp (\<lambda>Z::'a set. f \<union> EX' Z) \<inter> Collect P) \<Longrightarrow> P x) \<Longrightarrow> P a"
-    apply (erule EF_induct_prep)
-    apply assumption
-  by simp
+    by (erule EF_induct_prep, assumption, simp)
 qed
 
 lemma valEF_E: "M \<turnstile> EF f \<Longrightarrow> x \<in> init M \<Longrightarrow> x \<in> EF f"
 proof (simp add: check_def) 
   show "init M \<subseteq> {s::'a \<in> states M. s \<in> EF f} \<Longrightarrow> x \<in> init M \<Longrightarrow> x \<in> EF f"
-   apply (drule subsetD)
-   apply assumption
-    by simp
+    by blast
 qed
 
 lemma EF_step_star_rev[rule_format]: "x \<in> EF s \<Longrightarrow>  (\<exists> y \<in> s.  x  \<rightarrow>\<^sub>i* y)"
 proof (erule EF_induct)
   show "mono (\<lambda>Z::'a set. s \<union> EX' Z)"
-    apply (simp add: mono_def EX'_def)
-    by force
+    by (simp add: mono_def EX'_def, force)
 next show "\<And>x::'a. x \<in> s \<union> EX' (EF s \<inter> {x::'a. \<exists>y::'a\<in>s. x \<rightarrow>\<^sub>i* y}) \<Longrightarrow> \<exists>y::'a\<in>s. x \<rightarrow>\<^sub>i* y"
-apply (erule UnE)
-   apply (rule_tac x = x in bexI)
-    apply (simp add: state_transition_refl_def)
-   apply assumption
-  apply (simp add: EX'_def)
-  apply (erule bexE)
-  apply (erule IntE)
-  apply (drule CollectD)
-  apply (erule bexE)
-  apply (rule_tac x = xb in bexI)
-   apply (simp add: state_transition_refl_def)
-   apply (rule rtrancl_trans)
-    apply (rule r_into_rtrancl)
-    apply (rule CollectI)
-    apply simp
-  by assumption+
+    apply (erule UnE)
+    using state_transition_refl_def apply auto[1]
+    by (auto simp add: EX'_def state_transition_refl_def intro: converse_rtrancl_into_rtrancl)
 qed
 
 lemma EF_step_inv: "(I \<subseteq> {sa::'s :: state. (\<exists>i::'s\<in>I. i \<rightarrow>\<^sub>i* sa) \<and> sa \<in> EF s})  
          \<Longrightarrow> \<forall> x \<in> I. \<exists> y \<in> s. x \<rightarrow>\<^sub>i* y"
 proof (clarify)
   show "\<And>x::'s. I \<subseteq> {sa::'s. (\<exists>i::'s\<in>I. i \<rightarrow>\<^sub>i* sa) \<and> sa \<in> EF s} \<Longrightarrow> x \<in> I \<Longrightarrow> \<exists>y::'s\<in>s. x \<rightarrow>\<^sub>i* y"
-    apply (drule subsetD)
-    apply assumption
-    apply (drule CollectD)
-    apply (erule conjE)
-    by (erule EF_step_star_rev)
+    using EF_step_star_rev by fastforce
 qed
   
 subsubsection \<open>AG lemmas\<close> 
@@ -655,9 +505,7 @@ subsubsection \<open>AG lemmas\<close>
 lemma AG_in_lem:   "x \<in> AG s \<Longrightarrow> x \<in> s"  
 proof (simp add: AG_def gfp_def)
   show "\<exists>xa\<subseteq>s. xa \<subseteq> AX xa \<and> x \<in> xa \<Longrightarrow> x \<in> s"
-    apply (erule exE)
-    apply (erule conjE)+
-    by (erule subsetD, assumption)
+    by blast
 qed
 
 lemma AG_lem1: "x \<in> s \<and> x \<in> (AX (AG s)) \<Longrightarrow> x \<in> AG s"
@@ -665,12 +513,12 @@ proof (simp add: AG_def)
   show "x \<in> s \<and> x \<in> AX (gfp (\<lambda>Z::'a set. s \<inter> AX Z)) \<Longrightarrow> x \<in> gfp (\<lambda>Z::'a set. s \<inter> AX Z)"
   apply (subgoal_tac "gfp (\<lambda>Z::'a set. s \<inter> AX Z) =
                       s \<inter> (AX (gfp (\<lambda>Z::'a set. s \<inter> AX Z)))")
-  apply (erule ssubst)
-  apply simp
-  apply (rule def_gfp_unfold)
-  apply (rule reflexive)
-  apply (unfold mono_def AX_def)
-  by auto
+     apply (erule ssubst)
+     apply simp
+    apply (rule def_gfp_unfold)
+     apply (rule reflexive)
+    apply (unfold mono_def AX_def)
+    by auto
 qed
 
 lemma AG_lem2: "x \<in> AG s \<Longrightarrow> x \<in> (s \<inter> (AX (AG s)))"
@@ -688,36 +536,24 @@ qed
 lemma AG_lem3: "AG s = (s \<inter> (AX (AG s)))"    
 proof (rule equalityI) 
   show "AG s \<subseteq> s \<inter> AX (AG s)"
-    apply (rule subsetI)
-    by (erule AG_lem2)
+    using AG_lem2 by blast
   next show "s \<inter> AX (AG s) \<subseteq> AG s"
-    apply (rule subsetI)
-    apply (rule AG_lem1)
-    by simp
+      using AG_lem1 by blast
 qed
 
-lemma AG_step: "y \<rightarrow>\<^sub>i z \<Longrightarrow> y \<in> AG s \<Longrightarrow> z \<in> AG s"  
-proof (drule AG_lem2)
-  show "y \<rightarrow>\<^sub>i z \<Longrightarrow> y \<in> s \<inter> AX (AG s) \<Longrightarrow> z \<in> AG s"
-    apply (erule IntE)
-    apply (unfold AX_def)
-    apply simp
-    apply (erule subsetD)
-    by simp
-qed
+lemma AG_step: "y \<rightarrow>\<^sub>i z \<Longrightarrow> y \<in> AG s \<Longrightarrow> z \<in> AG s"
+  using AG_lem2 AX_def by blast  
 
 lemma AG_all_s: " x \<rightarrow>\<^sub>i* y \<Longrightarrow> x \<in> AG s \<Longrightarrow> y \<in> AG s"
 proof (simp add: state_transition_refl_def)
-  show "(x, y) \<in> {(x::'a, y::'a). x \<rightarrow>\<^sub>i y}\<^sup>* \<Longrightarrow> x \<in> AG s \<Longrightarrow> y \<in> AG s"
-    apply (erule rtrancl_induct) 
-  proof -
+  show "(x, y) \<in> {(x,y). x \<rightarrow>\<^sub>i y}\<^sup>* \<Longrightarrow> x \<in> AG s \<Longrightarrow> y \<in> AG s" 
+  proof (erule rtrancl_induct)
     show "x \<in> AG s \<Longrightarrow> x \<in> AG s" by assumption
   next show "\<And>(y::'a) z::'a.
        x \<in> AG s \<Longrightarrow>
-       (x, y) \<in> {(x::'a, y::'a). x \<rightarrow>\<^sub>i y}\<^sup>* \<Longrightarrow> 
-       (y, z) \<in> {(x::'a, y::'a). x \<rightarrow>\<^sub>i y} \<Longrightarrow> y \<in> AG s \<Longrightarrow> z \<in> AG s"
-      apply clarify
-      by (erule AG_step, assumption)
+       (x, y) \<in> {(x,y). x \<rightarrow>\<^sub>i y}\<^sup>* \<Longrightarrow> 
+       (y, z) \<in> {(x,y). x \<rightarrow>\<^sub>i y} \<Longrightarrow> y \<in> AG s \<Longrightarrow> z \<in> AG s"
+      by (simp add: AG_step)
   qed
 qed
 
@@ -744,33 +580,21 @@ proof (rule notI, simp add: check_def)
             hence "x \<in> s \<and> x \<in> -s"
             proof -
               have a6: "x \<in> s" using a5
-                apply (subgoal_tac "x \<in> AG s")
-                apply (erule AG_in_lem)
-                by simp
+                using AG_in_lem by blast
               moreover have "x \<in> -s" using a5
               proof -
-                have "x \<in> EF s" 
-                  apply (rule_tac y = x in EF_step_star)
-                  apply (simp add: state_transition_refl_def)
-                  by (rule a6)                  
+                have "x \<in> EF s"
+                  by (simp add: EF_lem2a calculation) 
                 thus "x \<in> -s" using a5
                 proof -
                   have "x \<in> EF (- s)" using a5
                     by simp
                   moreover from this obtain y where a7: "y \<in> - s \<and> x \<rightarrow>\<^sub>i* y" 
-                    apply (rotate_tac -1)
-                     apply (drule EF_step_star_rev)
-                    by blast
+                    using EF_step_star_rev by blast
                   moreover have "y \<in> AG s" using a7 a5
-                    apply (subgoal_tac "x \<in> AG s")
-                    apply (erule conjE)
-                     apply (drule AG_all_s)
-                      apply assumption+
-                    by simp
+                    using AG_all_s by blast
                   ultimately show "x \<in> -s" using a5
-                     apply (rotate_tac -1)
-                     apply (drule AG_in_lem)
-                     by blast
+                    using AG_in_lem by blast
                 qed
               qed
               ultimately show "x \<in> s \<and> x \<in> -s"
@@ -785,10 +609,8 @@ proof (rule notI, simp add: check_def)
       qed
     moreover have b: "? x. x : I" using a0
       by blast
-    moreover obtain x where "x \<in> I" 
-        apply (rule exE)
-         apply (rule b)
-      by simp
+    moreover obtain x where "x \<in> I"
+      using b by blast 
     ultimately show "False" using a0 a1 a2
       by blast
   qed
